Finalizing general (not prophecy specific) support for observations - Removing head of list of observations after each reduction step in definition of wp - Adding support for observations to state_interp and world - Applying Ralf's suggestions to previous commit (e.g. replacing /\ and -> with unicode characters)

theories/heap_lang/lang.v
@@ -108,7 +108,7 @@ Inductive val :=
 
 Bind Scope val_scope with val.
 
-Inductive observation := prophecy_observation_todo.
+Definition observation := Empty val.
 
 Fixpoint of_val (v : val) : expr :=
   match v with
