theories/program_logic/ownp.v
@@ -5,65 +5,67 @@ From iris.algebra Require Import auth.
 From iris.proofmode Require Import tactics classes.
 Set Default Proof Using "Type".
 
-Class ownPG' (Λstate : Type) (Σ : gFunctors) := OwnPG {
+Class ownPG' (Λstate Λobservation: Type) (Σ : gFunctors) := OwnPG {
   ownP_invG : invG Σ;
-  ownP_inG :> inG Σ (authR (optionUR (exclR (leibnizC Λstate))));
+  ownP_inG :> inG Σ (authR (optionUR (exclR (prodC (leibnizC Λstate) (leibnizC (list Λobservation))))));
   ownP_name : gname;
 }.
-Notation ownPG Λ Σ := (ownPG' (state Λ) Σ).
+Notation ownPG Λ Σ := (ownPG' (state Λ) (observation Λ) Σ).
 
-Instance ownPG_irisG `{ownPG' Λstate Σ} : irisG' Λstate Σ := {
+Instance ownPG_irisG `{ownPG' Λstate Λobservation Σ} : irisG' Λstate Λobservation Σ := {
   iris_invG := ownP_invG;
-  state_interp σ := own ownP_name (● (Excl' (σ:leibnizC Λstate)))
+  state_interp σ κs := own ownP_name (● (Excl' ((σ:leibnizC Λstate), (κs:leibnizC (list Λobservation)))))
 }.
 Global Opaque iris_invG.
 
-Definition ownPΣ (Λstate : Type) : gFunctors :=
+Definition ownPΣ (Λstate Λobservation : Type) : gFunctors :=
   #[invΣ;
-    GFunctor (authUR (optionUR (exclR (leibnizC Λstate))))].
+    GFunctor (authUR (optionUR (exclR (prodC (leibnizC Λstate) (leibnizC (list Λobservation))))))].
 
-Class ownPPreG' (Λstate : Type) (Σ : gFunctors) : Set := IrisPreG {
+Class ownPPreG' (Λstate Λobservation : Type) (Σ : gFunctors) : Set := IrisPreG {
   ownPPre_invG :> invPreG Σ;
-  ownPPre_inG :> inG Σ (authR (optionUR (exclR (leibnizC Λstate))))
+  ownPPre_inG :> inG Σ (authR (optionUR (exclR (prodC (leibnizC Λstate) (leibnizC (list Λobservation))))))
 }.
-Notation ownPPreG Λ Σ := (ownPPreG' (state Λ) Σ).
+Notation ownPPreG Λ Σ := (ownPPreG' (state Λ) (observation Λ) Σ).
 
-Instance subG_ownPΣ {Λstate Σ} : subG (ownPΣ Λstate) Σ → ownPPreG' Λstate Σ.
+Instance subG_ownPΣ {Λstate Λobservation Σ} : subG (ownPΣ Λstate Λobservation) Σ → ownPPreG' Λstate Λobservation Σ.
 Proof. solve_inG. Qed.
 
 (** Ownership *)
-Definition ownP `{ownPG' Λstate Σ} (σ : Λstate) : iProp Σ :=
-  own ownP_name (◯ (Excl' σ)).
+Definition ownP `{ownPG' Λstate Λobservation Σ} (σ : Λstate) (κs : list Λobservation) : iProp Σ :=
+  own ownP_name (◯ (Excl' (σ, κs))).
 Typeclasses Opaque ownP.
 Instance: Params (@ownP) 3.
 
 
 (* Adequacy *)
 Theorem ownP_adequacy Σ `{ownPPreG Λ Σ} s e σ φ :
-  (∀ `{ownPG Λ Σ}, ownP σ ⊢ WP e @ s; ⊤ {{ v, ⌜φ v⌝ }}) →
+  (∀ `{ownPG Λ Σ} κs, ownP σ κs ⊢ WP e @ s; ⊤ {{ v, ⌜φ v⌝ }}) →
   adequate s e σ (λ v _, φ v).
 Proof.
   intros Hwp. apply (wp_adequacy Σ _).
-  iIntros (?). iMod (own_alloc (● (Excl' (σ : leibnizC _)) ⋅ ◯ (Excl' σ)))
+  iIntros (? κs). iMod (own_alloc (● (Excl' (σ : leibnizC _, κs : leibnizC _)) ⋅ ◯ (Excl' (σ, κs))))
     as (γσ) "[Hσ Hσf]"; first done.
-  iModIntro. iExists (λ σ, own γσ (● (Excl' (σ:leibnizC _)))). iFrame "Hσ".
-  iApply (Hwp (OwnPG _ _ _ _ γσ)). by rewrite /ownP.
+  iModIntro. iExists (λ σ κs, own γσ (● (Excl' (σ:leibnizC _, κs:leibnizC _)))). iFrame "Hσ".
+  iApply (Hwp (OwnPG _ _ _ _ _ γσ)). by rewrite /ownP.
 Qed.
 
 Theorem ownP_invariance Σ `{ownPPreG Λ Σ} s e σ1 t2 σ2 φ :
-  (∀ `{ownPG Λ Σ},
-    ownP σ1 ={⊤}=∗ WP e @ s; ⊤ {{ _, True }} ∗ |={⊤,∅}=> ∃ σ', ownP σ' ∧ ⌜φ σ'⌝) →
+  (∀ `{ownPG Λ Σ} κs,
+    ownP σ1 κs ={⊤}=∗ WP e @ s; ⊤ {{ _, True }} ∗ |={⊤,∅}=> ∃ σ' κs', ownP σ' κs' ∧ ⌜φ σ'⌝) →
   rtc erased_step ([e], σ1) (t2, σ2) →
   φ σ2.
 Proof.
   intros Hwp Hsteps. eapply (wp_invariance Σ Λ s e σ1 t2 σ2 _)=> //.
-  iIntros (?). iMod (own_alloc (● (Excl' (σ1 : leibnizC _)) ⋅ ◯ (Excl' σ1)))
+  iIntros (? κs κs').
+  iMod (own_alloc (● (Excl' ((σ1 : leibnizC _, κs ++ κs' : leibnizC _))) ⋅ ◯ (Excl' (σ1, κs ++ κs'))))
     as (γσ) "[Hσ Hσf]"; first done.
-  iExists (λ σ, own γσ (● (Excl' (σ:leibnizC _)))). iFrame "Hσ".
-  iMod (Hwp (OwnPG _ _ _ _ γσ) with "[Hσf]") as "[$ H]"; first by rewrite /ownP.
-  iIntros "!> Hσ". iMod "H" as (σ2') "[Hσf %]". rewrite/ownP.
-  iDestruct (own_valid_2 with "Hσ Hσf")
-    as %[->%Excl_included%leibniz_equiv _]%auth_valid_discrete_2; auto.
+  iExists (λ σ κs', own γσ (● (Excl' (σ:leibnizC _, κs':leibnizC _)))). iFrame "Hσ".
+  iMod (Hwp (OwnPG _ _ _ _ _ γσ) with "[Hσf]") as "[$ H]"; first by rewrite /ownP.
+  iIntros "!> Hσ". iMod "H" as (σ2' κs'') "[Hσf %]". rewrite/ownP.
+  iDestruct (own_valid_2 with "Hσ Hσf") as %[Hp _]%auth_valid_discrete_2.
+  pose proof (Excl_included _ _ Hp) as Hp'. apply leibniz_equiv in Hp'. inversion Hp'; subst. auto.
+  (* TODO (MR) inline this proof in introduction pattern? *)
 Qed.
 
 
@@ -74,34 +76,36 @@ Section lifting.
   Implicit Types e : expr Λ.
   Implicit Types Φ : val Λ → iProp Σ.
 
-  Lemma ownP_eq σ1 σ2 : state_interp σ1 -∗ ownP σ2 -∗ ⌜σ1 = σ2⌝.
+  Lemma ownP_eq σ1 σ2 κs1 κs2 : state_interp σ1 κs1 -∗ ownP σ2 κs2 -∗ ⌜σ1 = σ2 ∧ κs1 = κs2⌝.
   Proof.
     iIntros "Hσ1 Hσ2"; rewrite/ownP.
-    by iDestruct (own_valid_2 with "Hσ1 Hσ2")
-      as %[->%Excl_included%leibniz_equiv _]%auth_valid_discrete_2.
+    iDestruct (own_valid_2 with "Hσ1 Hσ2")
+      as %[Hp _]%auth_valid_discrete_2.
+    pose proof (Excl_included _ _ Hp) as Hp'. apply leibniz_equiv in Hp'. inversion Hp'; subst. auto.
+  (* TODO (MR) inline this proof in introduction pattern? *)
   Qed.
-  Lemma ownP_twice σ1 σ2 : ownP σ1 ∗ ownP σ2 ⊢ False.
+  Lemma ownP_twice σ1 σ2 κs1 κs2 : ownP σ1 κs1 ∗ ownP σ2 κs2 ⊢ False.
   Proof. rewrite /ownP -own_op own_valid. by iIntros (?). Qed.
-  Global Instance ownP_timeless σ : Timeless (@ownP (state Λ) Σ _ σ).
+  Global Instance ownP_timeless σ κs : Timeless (@ownP (state Λ) (observation Λ) Σ _ σ κs).
   Proof. rewrite /ownP; apply _. Qed.
 
   Lemma ownP_lift_step s E Φ e1 :
-    (|={E,∅}=> ∃ σ1, ⌜if s is NotStuck then reducible e1 σ1 else to_val e1 = None⌝ ∗ ▷ ownP σ1 ∗
-      ▷ ∀ κ e2 σ2 efs, ⌜prim_step e1 σ1 κ e2 σ2 efs⌝ -∗ ownP σ2
+    (|={E,∅}=> ∃ σ1 κs, ⌜if s is NotStuck then reducible e1 σ1 else to_val e1 = None⌝ ∗ ▷ ownP σ1 κs ∗
+      ▷ ∀ κ κs' e2 σ2 efs, ⌜prim_step e1 σ1 κ e2 σ2 efs ∧ κs = cons_obs κ κs'⌝ -∗ ownP σ2 κs'
             ={∅,E}=∗ WP e2 @ s; E {{ Φ }} ∗ [∗ list] ef ∈ efs, WP ef @ s; ⊤ {{ _, True }})
     ⊢ WP e1 @ s; E {{ Φ }}.
   Proof.
     iIntros "H". destruct (to_val e1) as [v|] eqn:EQe1.
     - apply of_to_val in EQe1 as <-. iApply fupd_wp.
-      iMod "H" as (σ1) "[Hred _]"; iDestruct "Hred" as %Hred.
+      iMod "H" as (σ1 κs) "[Hred _]"; iDestruct "Hred" as %Hred.
       destruct s; last done. apply reducible_not_val in Hred.
       move: Hred; by rewrite to_of_val.
-    - iApply wp_lift_step; [done|]; iIntros (σ1) "Hσ".
-      iMod "H" as (σ1' ?) "[>Hσf H]". iDestruct (ownP_eq with "Hσ Hσf") as %->.
-      iModIntro; iSplit; [by destruct s|]; iNext; iIntros (κ e2 σ2 efs Hstep).
+    - iApply wp_lift_step; [done|]; iIntros (σ1 κs) "Hσ".
+      iMod "H" as (σ1' κs' ?) "[>Hσf H]". iDestruct (ownP_eq with "Hσ Hσf") as %[-> ->].
+      iModIntro; iSplit; [by destruct s|]; iNext; iIntros (κ κs'' e2 σ2 efs [Hstep ->]).
       rewrite /ownP; iMod (own_update_2 with "Hσ Hσf") as "[Hσ Hσf]".
-      { by apply auth_update, option_local_update,
-          (exclusive_local_update _ (Excl σ2)). }
+      { apply auth_update. apply option_local_update.
+          (exclusive_local_update _ (Excl (σ2, _))). }
       iFrame "Hσ". iApply ("H" with "[]"); eauto.
   Qed.
 
@@ -115,12 +119,12 @@ Section lifting.
       by rewrite to_of_val in Hnv.
     - iApply wp_lift_stuck; [done|]. iIntros (σ1) "Hσ".
       iMod "H" as (σ1') "(% & >Hσf)".
-      by iDestruct (ownP_eq with "Hσ Hσf") as %->.
+      by iDestruct (ownP_eq with "Hσ Hσf") as %→.
   Qed.
 
   Lemma ownP_lift_pure_step `{Inhabited (state Λ)} s E Φ e1 :
     (∀ σ1, if s is NotStuck then reducible e1 σ1 else to_val e1 = None) →
-    (∀ σ1 κ e2 σ2 efs, prim_step e1 σ1 κ e2 σ2 efs → κ = None /\ σ1 = σ2) →
+    (∀ σ1 κ e2 σ2 efs, prim_step e1 σ1 κ e2 σ2 efs → κ = None ∧ σ1 = σ2) →
     (▷ ∀ κ e2 efs σ, ⌜prim_step e1 σ κ e2 σ efs⌝ →
       WP e2 @ s; E {{ Φ }} ∗ [∗ list] ef ∈ efs, WP ef @ s; ⊤ {{ _, True }})
     ⊢ WP e1 @ s; E {{ Φ }}.
@@ -160,7 +164,7 @@ Section lifting.
   Proof.
     iIntros (? Hdet) "[Hσ1 Hσ2]"; iApply ownP_lift_atomic_step; try done.
     iFrame; iNext; iIntros (κ e2' σ2' efs') "% Hσ2'".
-    edestruct Hdet as (->&Hval&->). done. by rewrite Hval; iApply "Hσ2".
+    edestruct Hdet as (→&Hval&→). done. by rewrite Hval; iApply "Hσ2".
   Qed.
 
   Lemma ownP_lift_atomic_det_step_no_fork {s E e1} σ1 v2 σ2 :
@@ -175,17 +179,17 @@ Section lifting.
 
   Lemma ownP_lift_pure_det_step `{Inhabited (state Λ)} {s E Φ} e1 e2 efs :
     (∀ σ1, if s is NotStuck then reducible e1 σ1 else to_val e1 = None) →
-    (∀ σ1 κ e2' σ2 efs', prim_step e1 σ1 κ e2' σ2 efs' → κ = None /\ σ1 = σ2 ∧ e2 = e2' ∧ efs = efs')→
+    (∀ σ1 κ e2' σ2 efs', prim_step e1 σ1 κ e2' σ2 efs' → κ = None ∧ σ1 = σ2 ∧ e2 = e2' ∧ efs = efs')→
     ▷ (WP e2 @ s; E {{ Φ }} ∗ [∗ list] ef ∈ efs, WP ef @ s; ⊤{{ _, True }})
     ⊢ WP e1 @ s; E {{ Φ }}.
   Proof.
     iIntros (? Hpuredet) "?"; iApply ownP_lift_pure_step=>//.
-    naive_solver. by iNext; iIntros (κ e' efs' σ (->&_&->&->)%Hpuredet).
+    naive_solver. by iNext; iIntros (κ e' efs' σ (→&_&→&→)%Hpuredet).
   Qed.
 
   Lemma ownP_lift_pure_det_step_no_fork `{Inhabited (state Λ)} {s E Φ} e1 e2 :
     (∀ σ1, if s is NotStuck then reducible e1 σ1 else to_val e1 = None) →
-    (∀ σ1 κ e2' σ2 efs', prim_step e1 σ1 κ e2' σ2 efs' → κ = None /\ σ1 = σ2 ∧ e2 = e2' ∧ [] = efs') →
+    (∀ σ1 κ e2' σ2 efs', prim_step e1 σ1 κ e2' σ2 efs' → κ = None ∧ σ1 = σ2 ∧ e2 = e2' ∧ [] = efs') →
     ▷ WP e2 @ s; E {{ Φ }} ⊢ WP e1 @ s; E {{ Φ }}.
   Proof.
     intros. rewrite -(wp_lift_pure_det_step e1 e2 []) ?big_sepL_nil ?right_id; eauto.
@@ -226,7 +230,7 @@ Section ectx_lifting.
 
   Lemma ownP_lift_pure_head_step s E Φ e1 :
     (∀ σ1, head_reducible e1 σ1) →
-    (∀ σ1 κ e2 σ2 efs, head_step e1 σ1 κ e2 σ2 efs → κ = None /\ σ1 = σ2) →
+    (∀ σ1 κ e2 σ2 efs, head_step e1 σ1 κ e2 σ2 efs → κ = None ∧ σ1 = σ2) →
     (▷ ∀ κ e2 efs σ, ⌜head_step e1 σ κ e2 σ efs⌝ →
       WP e2 @ s; E {{ Φ }} ∗ [∗ list] ef ∈ efs, WP ef @ s; ⊤ {{ _, True }})
     ⊢ WP e1 @ s; E {{ Φ }}.
@@ -271,7 +275,7 @@ Section ectx_lifting.
 
   Lemma ownP_lift_pure_det_head_step {s E Φ} e1 e2 efs :
     (∀ σ1, head_reducible e1 σ1) →
-    (∀ σ1 κ e2' σ2 efs', head_step e1 σ1 κ e2' σ2 efs' → κ = None /\ σ1 = σ2 ∧ e2 = e2' ∧ efs = efs') →
+    (∀ σ1 κ e2' σ2 efs', head_step e1 σ1 κ e2' σ2 efs' → κ = None ∧ σ1 = σ2 ∧ e2 = e2' ∧ efs = efs') →
     ▷ (WP e2 @ s; E {{ Φ }} ∗ [∗ list] ef ∈ efs, WP ef @ s; ⊤ {{ _, True }})
     ⊢ WP e1 @ s; E {{ Φ }}.
   Proof using Hinh.
@@ -281,7 +285,7 @@ Section ectx_lifting.
 
   Lemma ownP_lift_pure_det_head_step_no_fork {s E Φ} e1 e2 :
     (∀ σ1, head_reducible e1 σ1) →
-    (∀ σ1 κ e2' σ2 efs', head_step e1 σ1 κ e2' σ2 efs' → κ = None /\ σ1 = σ2 ∧ e2 = e2' ∧ [] = efs') →
+    (∀ σ1 κ e2' σ2 efs', head_step e1 σ1 κ e2' σ2 efs' → κ = None ∧ σ1 = σ2 ∧ e2 = e2' ∧ [] = efs') →
     ▷ WP e2 @ s; E {{ Φ }} ⊢ WP e1 @ s; E {{ Φ }}.
   Proof using Hinh.
     iIntros (??) "H". iApply ownP_lift_pure_det_step_no_fork; eauto.
