theories/heap_lang/total_adequacy.v
@@ -4,12 +4,15 @@ From iris.heap_lang Require Import proofmode notation.
 From iris.proofmode Require Import tactics.
 Set Default Proof Using "Type".
 
+(* TODO (MR) re-introduce lemma after we prove twp_total *)
+(*
 Definition heap_total Σ `{heapPreG Σ} s e σ φ :
   (∀ `{heapG Σ}, WP e @ s; ⊤ [{ v, ⌜φ v⌝ }]%I) →
   sn erased_step ([e], σ).
 Proof.
-  intros Hwp; eapply (twp_total _ _); iIntros (?) "".
+  intros Hwp; eapply (twp_total _ _) with (κs := []); iIntros (?) "".
   iMod (gen_heap_init σ) as (?) "Hh".
-  iModIntro. iExists gen_heap_ctx; iFrame.
+  iModIntro. iExists (fun σ _ => gen_heap_ctx σ); iFrame.
   iApply (Hwp (HeapG _ _ _)).
 Qed.
+*)
