theories/program_logic/total_ectx_lifting.v
@@ -14,21 +14,21 @@ Hint Resolve head_prim_reducible head_reducible_prim_step.
 
 Lemma twp_lift_head_step {s E Φ} e1 :
   to_val e1 = None →
-  (∀ σ1, state_interp σ1 ={E,∅}=∗
+  (∀ σ1 κs, state_interp σ1 κs ={E,∅}=∗
     ⌜head_reducible e1 σ1⌝ ∗
-    ∀ κ e2 σ2 efs, ⌜head_step e1 σ1 κ e2 σ2 efs⌝ ={∅,E}=∗
-      state_interp σ2 ∗ WP e2 @ s; E [{ Φ }] ∗ [∗ list] ef ∈ efs, WP ef @ s; ⊤ [{ _, True }])
+    ∀ κ κs' e2 σ2 efs, ⌜head_step e1 σ1 κ e2 σ2 efs ∧ κs = cons_obs κ κs'⌝ ={∅,E}=∗
+      state_interp σ2 κs' ∗ WP e2 @ s; E [{ Φ }] ∗ [∗ list] ef ∈ efs, WP ef @ s; ⊤ [{ _, True }])
   ⊢ WP e1 @ s; E [{ Φ }].
 Proof.
-  iIntros (?) "H". iApply (twp_lift_step _ E)=>//. iIntros (σ1) "Hσ".
+  iIntros (?) "H". iApply (twp_lift_step _ E)=>//. iIntros (σ1 κs) "Hσ".
   iMod ("H" $! σ1 with "Hσ") as "[% H]"; iModIntro.
-  iSplit; [destruct s; auto|]. iIntros (κ e2 σ2 efs) "%".
+  iSplit; [destruct s; auto|]. iIntros (κ κs' e2 σ2 efs [Hstep ->]).
   iApply "H". by eauto.
 Qed.
 
 Lemma twp_lift_pure_head_step {s E Φ} e1 :
   (∀ σ1, head_reducible e1 σ1) →
-  (∀ σ1 κ e2 σ2 efs, head_step e1 σ1 κ e2 σ2 efs → κ = None /\ σ1 = σ2) →
+  (∀ σ1 κ e2 σ2 efs, head_step e1 σ1 κ e2 σ2 efs → κ = None ∧ σ1 = σ2) →
   (|={E}=> ∀ κ e2 efs σ, ⌜head_step e1 σ κ e2 σ efs⌝ →
     WP e2 @ s; E [{ Φ }] ∗ [∗ list] ef ∈ efs, WP ef @ s; ⊤ [{ _, True }])
   ⊢ WP e1 @ s; E [{ Φ }].
@@ -39,36 +39,36 @@ Qed.
 
 Lemma twp_lift_atomic_head_step {s E Φ} e1 :
   to_val e1 = None →
-  (∀ σ1, state_interp σ1 ={E}=∗
+  (∀ σ1 κs, state_interp σ1 κs ={E}=∗
     ⌜head_reducible e1 σ1⌝ ∗
-    ∀ κ e2 σ2 efs, ⌜head_step e1 σ1 κ e2 σ2 efs⌝ ={E}=∗
-      state_interp σ2 ∗
+    ∀ κ κs' e2 σ2 efs, ⌜head_step e1 σ1 κ e2 σ2 efs ∧ κs = cons_obs κ κs'⌝ ={E}=∗
+      state_interp σ2 κs'∗
       from_option Φ False (to_val e2) ∗ [∗ list] ef ∈ efs, WP ef @ s; ⊤ [{ _, True }])
   ⊢ WP e1 @ s; E [{ Φ }].
 Proof.
   iIntros (?) "H". iApply twp_lift_atomic_step; eauto.
-  iIntros (σ1) "Hσ1". iMod ("H" $! σ1 with "Hσ1") as "[% H]"; iModIntro.
-  iSplit; first by destruct s; auto. iIntros (κ e2 σ2 efs) "%". iApply "H"; eauto.
+  iIntros (σ1 κs) "Hσ1". iMod ("H" $! σ1 with "Hσ1") as "[% H]"; iModIntro.
+  iSplit; first by destruct s; auto. iIntros (κ κs' e2 σ2 efs [Hstep ->]). iApply "H"; eauto.
 Qed.
 
 Lemma twp_lift_atomic_head_step_no_fork {s E Φ} e1 :
   to_val e1 = None →
-  (∀ σ1, state_interp σ1 ={E}=∗
+  (∀ σ1 κs, state_interp σ1 κs ={E}=∗
     ⌜head_reducible e1 σ1⌝ ∗
-    ∀ κ e2 σ2 efs, ⌜head_step e1 σ1 κ e2 σ2 efs⌝ ={E}=∗
-      ⌜efs = []⌝ ∗ state_interp σ2 ∗ from_option Φ False (to_val e2))
+    ∀ κ κs' e2 σ2 efs, ⌜head_step e1 σ1 κ e2 σ2 efs ∧ κs = cons_obs κ κs'⌝ ={E}=∗
+      ⌜efs = []⌝ ∗ state_interp σ2 κs' ∗ from_option Φ False (to_val e2))
   ⊢ WP e1 @ s; E [{ Φ }].
 Proof.
   iIntros (?) "H". iApply twp_lift_atomic_head_step; eauto.
-  iIntros (σ1) "Hσ1". iMod ("H" $! σ1 with "Hσ1") as "[$ H]"; iModIntro.
-  iIntros (κ v2 σ2 efs) "%".
-  iMod ("H" $! κ v2 σ2 efs with "[# //]") as "(% & $ & $)"; subst; auto.
+  iIntros (σ1 κs) "Hσ1". iMod ("H" $! σ1 with "Hσ1") as "[$ H]"; iModIntro.
+  iIntros (κ κs' v2 σ2 efs [Hstep ->]).
+  iMod ("H" $! κ κs' v2 σ2 efs with "[# //]") as "(% & $ & $)"; subst; auto.
 Qed.
 
 Lemma twp_lift_pure_det_head_step {s E Φ} e1 e2 efs :
   (∀ σ1, head_reducible e1 σ1) →
   (∀ σ1 κ e2' σ2 efs',
-    head_step e1 σ1 κ e2' σ2 efs' → κ = None /\ σ1 = σ2 ∧ e2 = e2' ∧ efs = efs') →
+    head_step e1 σ1 κ e2' σ2 efs' → κ = None ∧ σ1 = σ2 ∧ e2 = e2' ∧ efs = efs') →
   (|={E}=> WP e2 @ s; E [{ Φ }] ∗ [∗ list] ef ∈ efs, WP ef @ s; ⊤ [{ _, True }])
   ⊢ WP e1 @ s; E [{ Φ }].
 Proof using Hinh. eauto using twp_lift_pure_det_step. Qed.
@@ -77,7 +77,7 @@ Lemma twp_lift_pure_det_head_step_no_fork {s E Φ} e1 e2 :
   to_val e1 = None →
   (∀ σ1, head_reducible e1 σ1) →
   (∀ σ1 κ e2' σ2 efs',
-    head_step e1 σ1 κ e2' σ2 efs' → κ = None /\ σ1 = σ2 ∧ e2 = e2' ∧ [] = efs') →
+    head_step e1 σ1 κ e2' σ2 efs' → κ = None ∧ σ1 = σ2 ∧ e2 = e2' ∧ [] = efs') →
   WP e2 @ s; E [{ Φ }] ⊢ WP e1 @ s; E [{ Φ }].
 Proof using Hinh.
   intros. rewrite -(twp_lift_pure_det_step e1 e2 []) /= ?right_id; eauto.
