theories/program_logic/total_lifting.v
@@ -13,14 +13,15 @@ Implicit Types Φ : val Λ → iProp Σ.
 
 Lemma twp_lift_step s E Φ e1 :
   to_val e1 = None →
-  (∀ σ1, state_interp σ1 ={E,∅}=∗
+  (∀ σ1 κs, state_interp σ1 κs ={E,∅}=∗
     ⌜if s is NotStuck then reducible e1 σ1 else True⌝ ∗
-    ∀ κ e2 σ2 efs, ⌜prim_step e1 σ1 κ e2 σ2 efs⌝ ={∅,E}=∗
-      state_interp σ2 ∗ WP e2 @ s; E [{ Φ }] ∗ [∗ list] ef ∈ efs, WP ef @ s; ⊤ [{ _, True }])
+    ∀ κ κs' e2 σ2 efs, ⌜prim_step e1 σ1 κ e2 σ2 efs ∧ κs = cons_obs κ κs'⌝ ={∅,E}=∗
+      state_interp σ2 κs' ∗ WP e2 @ s; E [{ Φ }] ∗ [∗ list] ef ∈ efs, WP ef @ s; ⊤ [{ _, True }])
   ⊢ WP e1 @ s; E [{ Φ }].
 Proof. by rewrite twp_unfold /twp_pre=> ->. Qed.
 
 (** Derived lifting lemmas. *)
+
 Lemma twp_lift_pure_step `{Inhabited (state Λ)} s E Φ e1 :
   (∀ σ1, reducible e1 σ1) →
   (∀ σ1 κ e2 σ2 efs, prim_step e1 σ1 κ e2 σ2 efs → κ = None /\ σ1 = σ2) →
@@ -30,9 +31,9 @@ Lemma twp_lift_pure_step `{Inhabited (state Λ)} s E Φ e1 :
 Proof.
   iIntros (Hsafe Hstep) "H". iApply twp_lift_step.
   { eapply reducible_not_val, (Hsafe inhabitant). }
-  iIntros (σ1) "Hσ". iMod "H".
+  iIntros (σ1 κs) "Hσ". iMod "H".
   iMod fupd_intro_mask' as "Hclose"; last iModIntro; first set_solver.
-  iSplit; [by destruct s|]; iIntros (κ e2 σ2 efs ?).
+  iSplit; [by destruct s|]; iIntros (κ κs' e2 σ2 efs [Hstep' ->]).
   destruct (Hstep σ1 κ e2 σ2 efs); auto; subst.
   iMod "Hclose" as "_". iFrame "Hσ". iApply "H"; auto.
 Qed.
@@ -41,18 +42,18 @@ Qed.
    use the generic lemmas here. *)
 Lemma twp_lift_atomic_step {s E Φ} e1 :
   to_val e1 = None →
-  (∀ σ1, state_interp σ1 ={E}=∗
+  (∀ σ1 κs, state_interp σ1 κs ={E}=∗
     ⌜if s is NotStuck then reducible e1 σ1 else True⌝ ∗
-    ∀ κ e2 σ2 efs, ⌜prim_step e1 σ1 κ e2 σ2 efs⌝ ={E}=∗
-      state_interp σ2 ∗
+    ∀ κ κs' e2 σ2 efs, ⌜prim_step e1 σ1 κ e2 σ2 efs ∧ κs = cons_obs κ κs'⌝ ={E}=∗
+      state_interp σ2 κs' ∗
       from_option Φ False (to_val e2) ∗ [∗ list] ef ∈ efs, WP ef @ s; ⊤ [{ _, True }])
   ⊢ WP e1 @ s; E [{ Φ }].
 Proof.
-  iIntros (?) "H". iApply (twp_lift_step _ E _ e1)=>//; iIntros (σ1) "Hσ1".
+  iIntros (?) "H". iApply (twp_lift_step _ E _ e1)=>//; iIntros (σ1 κs) "Hσ1".
   iMod ("H" $! σ1 with "Hσ1") as "[$ H]".
   iMod (fupd_intro_mask' E ∅) as "Hclose"; first set_solver.
-  iIntros "!>" (κ e2 σ2 efs) "%". iMod "Hclose" as "_".
-  iMod ("H" $! κ e2 σ2 efs with "[#]") as "($ & HΦ & $)"; first by eauto.
+  iIntros "!>" (κ κs' e2 σ2 efs) "%". iMod "Hclose" as "_".
+  iMod ("H" $! κ κs' e2 σ2 efs with "[#]") as "($ & HΦ & $)"; first by eauto.
   destruct (to_val e2) eqn:?; last by iExFalso.
   iApply twp_value; last done. by apply of_to_val.
 Qed.
@@ -76,4 +77,5 @@ Proof.
   iIntros ([??] Hφ) "HWP".
   iApply (twp_lift_pure_det_step with "[HWP]"); [eauto|naive_solver|auto].
 Qed.
+
 End lifting.
